extracted Specs.SeqExt.filter (& related) into separate Seq.Filter.*

src/Flutterbye.Seq.Filter.fsi
@@ -1,0 +1,60 @@
+(*--build-config
+   options:--admit_fsi FStar.Seq --admit_fsi Flutterbye.Seq.Mem;
+   other-files:seq.fsi Flutterbye.Seq.Mem.fsi
+--*)
+
+// $legal:614:
+//
+// Copyright 2015 Michael Lowell Roberts
+//
+// Licensed under the Apache License, Version 2.0 (the "License");
+// you may not use this file except in compliance with the License.
+// You may obtain a copy of the License at
+//
+//     http://www.apache.org/licenses/LICENSE-2.0
+//
+// Unless required by applicable law or agreed to in writing, software
+// distributed under the License is distributed on an "AS IS" BASIS,
+// WITHOUT WARRANTIES OR CONDITIONS OF ANY KIND, either express or implied.
+// See the License for the specific language governing permissions and
+// limitations under the License.
+//
+// ,$
+
+module Flutterbye.Seq.Filter
+   open FStar.Seq
+   open Flutterbye.Seq.Mem
+
+   val filter:
+      ('a -> Tot bool)
+         // predicate; if false, then the element is discarded from the
+         // sequence.
+      -> seq 'a // input sequence
+      -> Tot (seq 'a) // output sequence
+
+   val lemma__predicate:
+      p: ('a -> Tot bool)
+      -> s: seq 'a
+      -> i: nat{i < length (filter p s)}
+      -> Lemma
+         (requires (True))
+         (ensures (p (index (filter p s) i)))
+         [SMTPat (index (filter p s) i)]
+
+   val lemma__length:
+      p: ('a -> Tot bool)
+      -> s: seq 'a
+      -> Lemma
+         (requires (True))
+         (ensures (length (filter p s) <= length s))
+         [SMTPat (length (filter p s))]
+
+   val lemma__preserves_mem:
+      p: ('a -> Tot bool) ->
+      s: seq 'a ->
+      Lemma
+         (requires (True))
+         (ensures
+            (forall i.
+               0 <= i && i < length (filter p s)
+               ==> mem s (index (filter p s) i)))
