src/specs/seqext.fst
@@ -1,6 +1,6 @@
 (*--build-config
-   options:--admit_fsi FStar.Seq --admit_fsi Flutterbye.Seq.Find --admit_fsi Flutterbye.Seq.Mem;
-   other-files:seq.fsi ../Flutterbye.Seq.Find.fsi ../Flutterbye.Seq.Mem.fsi seqext.fsi
+   options:--admit_fsi FStar.Seq --admit_fsi Flutterbye.Seq.Find --admit_fsi Flutterbye.Seq.Mem --admit_fsi Flutterbye.Seq.Filter;
+   other-files:seq.fsi ../Flutterbye.Seq.Find.fsi ../Flutterbye.Seq.Mem.fsi ../Flutterbye.Seq.Filter.fsi seqext.fsi
 --*)
 
 // $legal:614:
@@ -25,129 +25,13 @@ module Flutterbye.Specs.SeqExt
    open FStar.Seq
    open Flutterbye.Seq.Find
    open Flutterbye.Seq.Mem
-
-   val __filter__loop:
-      // predicate; if false, then the element is discarded from the sequence.
-      ('a -> Tot bool)
-      // input sequence
-      -> s: seq 'a
-      // index of element being reduced with (length s) as representing
-      // the base case.
-      -> i: nat{i <= length s}
-      // accumulator; in this case, the output sequence.
-      -> c: seq 'a
-      -> Tot (seq 'a)
-         (decreases (length s - i))
-   let rec __filter__loop p s i c =
-      if i = length s then
-         c
-      else
-         let a = index s i in
-         let c' =
-            if p a then
-               append c (create 1 a)
-            else
-               c in
-         __filter__loop p s (i + 1) c'
-
-   let filter p s =
-      __filter__loop p s 0 createEmpty
-
-   val __lemma_filter__loop__length:
-      p: ('a -> Tot bool) ->
-      s: seq 'a ->
-      i: nat{i <= length s} ->
-      c: seq 'a ->
-      Lemma
-         (requires (length c <= i))
-         (ensures (length (__filter__loop p s i c) <= length s))
-         (decreases (length s - i))
-   let rec __lemma_filter__loop__length p s i c =
-      if i = length s then
-         ()
-      else
-         let a = index s i in
-         let c' =
-            if p a then
-               append c (create 1 a)
-            else
-               c in
-         __lemma_filter__loop__length p s (i + 1) c'
-
-   val lemma_filter__length:
-      p: ('a -> Tot bool)
-      -> s: seq 'a
-      -> Lemma
-         (requires (True))
-         (ensures (length (filter p s) <= length s))
-         [SMTPat (length (filter p s))]
-   let lemma_filter__length p s =
-      __lemma_filter__loop__length p s 0 createEmpty
-
-   val __lemma_filter__loop__admission:
-      p: ('a -> Tot bool)
-      -> s: seq 'a
-      -> i: nat{i <= length s}
-      // accumulator-- in this case, a filtered sequence being constructed.
-      -> c: seq 'a
-      // free variable (forall)
-      -> j: nat
-      -> Lemma
-         (requires
-            (forall k.
-               0 <= k && k < length c ==> p (index c k)))
-         (ensures
-            (j < length (__filter__loop p s i c)
-            ==> p (index (__filter__loop p s i c) j)))
-         (decreases (length s - i))
-   let rec __lemma_filter__loop__admission p s i c j =
-      if i = length s then
-         ()
-      else
-         let a = index s i in
-         let c' =
-            if p a then
-               append c (create 1 a)
-            else
-               c in
-         __lemma_filter__loop__admission p s (i + 1) c' j
-
-   let lemma_filter__admission p s i =
-      __lemma_filter__loop__admission p s 0 createEmpty i
-
-   val __lemma_filter__loop__mem:
-      p: ('a -> Tot bool)
-      -> s: seq 'a
-      -> i: nat{i <= length s}
-      -> c: seq 'a
-      -> Lemma
-         (requires
-            (forall j.
-               (0 <= j && j < length c) ==> (mem s (index c j))))
-         (ensures
-            (forall j.
-               (0 <= j && j < length (__filter__loop p s i c)) ==> (mem s (index (__filter__loop p s i c) j))))
-         (decreases (length s - i))
-   let rec __lemma_filter__loop__mem p s i c =
-      if i = length s then
-         ()
-      else
-         let a = index s i in
-         let c' =
-            if p a then
-               append c (create 1 a)
-            else
-               c in
-         __lemma_filter__loop__mem p s (i + 1) c'
-
-   let lemma_filter__mem p s =
-      __lemma_filter__loop__mem p s 0 createEmpty
+   open Flutterbye.Seq.Filter
 
    let count p s =
       length (filter p s)
 
    let lemma_count__length p s =
-      lemma_filter__length p s
+      Flutterbye.Seq.Filter.lemma__length p s
 
    let insert s i a =
       let l = slice s 0 i in
