src/Flutterbye.Seq.Filter.fst
@@ -1,0 +1,136 @@
+(*--build-config
+   options:--admit_fsi FStar.Seq --admit_fsi Flutterbye.Seq.Mem;
+   other-files:seq.fsi Flutterbye.Seq.Mem.fsi
+--*)
+
+// $legal:614:
+//
+// Copyright 2015 Michael Lowell Roberts
+//
+// Licensed under the Apache License, Version 2.0 (the "License");
+// you may not use this file except in compliance with the License.
+// You may obtain a copy of the License at
+//
+//     http://www.apache.org/licenses/LICENSE-2.0
+//
+// Unless required by applicable law or agreed to in writing, software
+// distributed under the License is distributed on an "AS IS" BASIS,
+// WITHOUT WARRANTIES OR CONDITIONS OF ANY KIND, either express or implied.
+// See the License for the specific language governing permissions and
+// limitations under the License.
+//
+// ,$
+
+module Flutterbye.Seq.Filter
+   open FStar.Seq
+   open Flutterbye.Seq.Mem
+
+   val filter__loop:
+      // predicate; if false, then the element is discarded from the sequence.
+      ('a -> Tot bool)
+      // input sequence
+      -> s: seq 'a
+      // index of element being reduced with (length s) as representing
+      // the base case.
+      -> i: nat{i <= length s}
+      // accumulator; in this case, the output sequence.
+      -> c: seq 'a
+      -> Tot (seq 'a)
+         (decreases (length s - i))
+   let rec filter__loop p s i c =
+      if i = length s then
+         c
+      else
+         let a = index s i in
+         let c' =
+            if p a then
+               append c (create 1 a)
+            else
+               c in
+         filter__loop p s (i + 1) c'
+
+   let filter p s =
+      filter__loop p s 0 createEmpty
+
+   val lemma__length__loop:
+      p: ('a -> Tot bool) ->
+      s: seq 'a ->
+      i: nat{i <= length s} ->
+      c: seq 'a ->
+      Lemma
+         (requires (length c <= i))
+         (ensures (length (filter__loop p s i c) <= length s))
+         (decreases (length s - i))
+   let rec lemma__length__loop p s i c =
+      if i = length s then
+         ()
+      else
+         let a = index s i in
+         let c' =
+            if p a then
+               append c (create 1 a)
+            else
+               c in
+         lemma__length__loop p s (i + 1) c'
+
+   let lemma__length p s =
+      lemma__length__loop p s 0 createEmpty
+
+   val lemma__predicate__loop:
+      p: ('a -> Tot bool)
+      -> s: seq 'a
+      -> i: nat{i <= length s}
+      // accumulator-- in this case, a filtered sequence being constructed.
+      -> c: seq 'a
+      // free variable (forall)
+      -> j: nat
+      -> Lemma
+         (requires
+            (forall k.
+               0 <= k && k < length c ==> p (index c k)))
+         (ensures
+            (j < length (filter__loop p s i c)
+            ==> p (index (filter__loop p s i c) j)))
+         (decreases (length s - i))
+   let rec lemma__predicate__loop p s i c j =
+      if i = length s then
+         ()
+      else
+         let a = index s i in
+         let c' =
+            if p a then
+               append c (create 1 a)
+            else
+               c in
+         lemma__predicate__loop p s (i + 1) c' j
+
+   let lemma__predicate p s i =
+      lemma__predicate__loop p s 0 createEmpty i
+
+   val lemma__mem__loop:
+      p: ('a -> Tot bool)
+      -> s: seq 'a
+      -> i: nat{i <= length s}
+      -> c: seq 'a
+      -> Lemma
+         (requires
+            (forall j.
+               (0 <= j && j < length c) ==> (mem s (index c j))))
+         (ensures
+            (forall j.
+               (0 <= j && j < length (filter__loop p s i c)) ==> (mem s (index (filter__loop p s i c) j))))
+         (decreases (length s - i))
+   let rec lemma__mem__loop p s i c =
+      if i = length s then
+         ()
+      else
+         let a = index s i in
+         let c' =
+            if p a then
+               append c (create 1 a)
+            else
+               c in
+         lemma__mem__loop p s (i + 1) c'
+
+   let lemma__mem p s =
+      lemma__mem__loop p s 0 createEmpty
